

④ $A = \begin{pmatrix} 1 & 2 & 3 \\ 4 & 5 & 6 \\ 3 & 2 & 2 \end{pmatrix}$ Método de Crout

$$L = \begin{pmatrix} L_{11} & 0 & 0 \\ L_{21} & L_{22} & 0 \\ L_{31} & L_{32} & L_{33} \end{pmatrix}, U = \begin{pmatrix} 1 & u_{12} & u_{13} \\ 0 & 1 & u_{23} \\ 0 & 0 & 1 \end{pmatrix}$$

$$\begin{aligned} L_{11} &= 1 & u_{12} &= \frac{2}{1} = 2 & L_{22} &= 5 - 4 \cdot 2 = -3 \\ L_{21} &= 4 & u_{13} &= \frac{3}{1} = 3 & L_{32} &= 2 - 3 \cdot 2 = -4 \\ L_{31} &= 3 & & & & \end{aligned}$$

$$u_{23} = \frac{a_{23} - L_{2,3} \cdot u_{13}}{L_{2,2}} = \frac{6 - 4 \cdot 3}{-3} = 2$$

$$L_{33} = a_{3,3} - (L_{3,1} \cdot u_{1,3} + L_{3,2} \cdot u_{2,3}) = 2 - (3 \cdot 3 + (-4) \cdot (2)) = 1$$

$$L = \begin{pmatrix} 1 & 0 & 0 \\ 4 & -3 & 0 \\ 3 & -4 & 1 \end{pmatrix}, U = \begin{pmatrix} 1 & 2 & 3 \\ 0 & 1 & 2 \\ 0 & 0 & 1 \end{pmatrix} \quad L \times U = \begin{pmatrix} 1 & 2 & 3 \\ 4 & 5 & 6 \\ 3 & 2 & 2 \end{pmatrix}$$